Proof that x_t at the end of the proof is x^(t+1).

BG_formalization.thy
@@ -1,8 +1,7 @@
 theory BG_formalization imports
   Main
-  CryptHOL.CryptHOL
   "Crypto_Standards.Words"
-  
+  "CryptHOL.CryptHOL"
 begin
 
 section "Introduction"
@@ -43,16 +42,15 @@ text "We define the loop in the encryption as a recursive function. This functio
 -bit conversion function as a parameter:"
 
 fun enc_loop_func 
-  :: "((nat => bitstring) \<times> nat \<times> nat \<times> bitstring list) \<Rightarrow> bitstring list \<Rightarrow> nat \<Rightarrow> (bitstring list \<times> nat)" 
+  :: "((nat  => bitstring) \<times> nat \<times> nat \<times> bitstring list) \<Rightarrow> bitstring list \<Rightarrow> nat \<Rightarrow> (bitstring list \<times> nat)" 
   where
    "enc_loop_func (f, n, h, []) c_acc x = (c_acc, x)" |
-   "enc_loop_func (f, n, h, (m_i # m_rest)) c_acc x = do
-        {
-        let x_i = x * x mod n;
-        let p_i = f (x_i mod 2^h);
-        let c_i = m_i [\<oplus>] p_i;
+   "enc_loop_func (f, n, h, (m_i # m_rest)) c_acc x =
+        (let x_i = x * x mod n in
+        let p_i = f (x_i mod 2^h) in
+        let c_i = m_i [\<oplus>] p_i in
         enc_loop_func (f, n, h, m_rest) (c_i # c_acc) x_i
-        }"
+        )"
 
 
 text "A simple function to convert a bit represented by a natural number to a bit represented by a 
@@ -68,28 +66,197 @@ text "The function gives False for anything other than True."
 
 text "We finally define a function to convert a natural number to a bitstring, with the help of 
 nat_to_bits."
-definition nat_to_bitstring :: "nat \<Rightarrow> bitstring" where 
-  "nat_to_bitstring = (\<lambda>n. map (nat_to_bit) (nat_to_bits n))"
+definition nat_to_bitstring :: "nat \<Rightarrow> nat \<Rightarrow> bitstring" where 
+  "nat_to_bitstring = (\<lambda>l n. map (nat_to_bit) (nat_to_bits_len n l))"
 
 text "Abstracting away from accumulators and conversion functions:"
 fun enc_loop 
    :: "(nat \<times> nat \<times> bitstring list) \<Rightarrow> nat \<Rightarrow> (bitstring list \<times> nat)" 
    where
    "enc_loop (n, h, m) x 
-    = enc_loop_func (nat_to_bitstring, n, h, m) [] x "
+    = enc_loop_func (nat_to_bitstring h, n, h, m) [] x"
 
 text "At last, the encryption function:"
 definition encrypt :: "nat \<Rightarrow> bitstring \<Rightarrow> nat \<Rightarrow> (bitstring list \<times> nat)" where
-  "encrypt n m r = 
-  do {
-  let h = nat \<lfloor>log 2 (log 2 n)\<rfloor>;
-  let t = \<lceil>h / (length m)\<rceil>;
-  let m_l = split m h;
-  let (x_0 :: nat) = (r * r) mod n;
-  let (c, x_t) = enc_loop (n, h, m_l) x_0;
-  let x_t' = x_t * x_t mod n;
-  (c, x_t')}"
+  "encrypt n m r = (
+  let h = nat \<lfloor>log 2 (log 2 n)\<rfloor> in 
+  let m_l = split m h in 
+  let (x_0 :: nat) = (r * r) mod n in 
+  let (c, x_t) = enc_loop (n, h, m_l) x_0 in 
+  let x_t' = x_t * x_t mod n in 
+  (c, x_t'))"
+
+
+text "An alternate definition of floor log:"
+
+fun floor_nat_log_rec :: "nat \<Rightarrow> nat \<Rightarrow> nat \<Rightarrow> nat" where
+  "floor_nat_log_rec 0 n acc = 0" |
+  "floor_nat_log_rec (Suc 0) n acc = 0" |
+  "floor_nat_log_rec base 0 0 = 0" | 
+  "floor_nat_log_rec base 0 (Suc acc) = acc" | 
+  "floor_nat_log_rec base (Suc n) acc 
+    = floor_nat_log_rec base ((Suc n) div base) (Suc acc)"
+
+definition floor_nat_log :: "nat \<Rightarrow> nat \<Rightarrow> nat" where
+  "floor_nat_log base n = floor_nat_log_rec base n 0" 
+
+definition encrypt_discrete_log :: "nat \<Rightarrow> bitstring \<Rightarrow> nat \<Rightarrow> (bitstring list \<times> nat)" where
+  "encrypt_discrete_log n m r = (
+  let h = (floor_nat_log 2 (floor_nat_log 2 n)) in 
+  let m_l = split m h in 
+  let (x_0 :: nat) = (r * r) mod n in 
+  let (c, x_t) = enc_loop (n, h, m_l) x_0 in 
+  let x_t' = x_t * x_t mod n in 
+  (c, x_t'))"
+
+
+text "now the decryption..."
+
+fun calculate_exponent :: "nat \<Rightarrow> nat \<Rightarrow> nat" where 
+  "calculate_exponent t p = 
+    (let d_p = ((Suc p) div 4)^(Suc t) mod (p-1) in d_p)"
+
+fun merge_list :: "'a list list => 'a list" where
+  "merge_list [] = []" |
+  "merge_list (x # xs) = x @ (merge_list xs)"
+
+definition decrypt :: "nat \<Rightarrow> nat \<Rightarrow> (bitstring list \<times> nat) \<Rightarrow> bitstring" where
+  "decrypt p q tup = (case tup of (c, x) \<Rightarrow> 
+   (let u_p = x ^ (calculate_exponent (length c) p) in
+    let u_q = x ^ (calculate_exponent (length c) q) in
+    let ((r_p, r_q), _) = euclid_ext p q in
+    let x_0 = nat (u_p * r_p * p + u_q * r_q * q mod (p * q)) in
+    let (m, x') = enc_loop (p * q, (nat \<lfloor>log 2 (log 2 (p * q))\<rfloor>) , c) x_0 in
+    merge_list m))"
+
+text "Correctness proof"
+
+lemma enc_loop_func_exp: 
+  assumes "n > 0" "h > 0" "x < n"
+  shows "snd (enc_loop_func (nat_to_bitstring h, n, h, m) c x) = x ^ (2 ^ (length m)) mod n"
+  using assms
+proof (induction m arbitrary: x c)
+  case Nil
+  then have "(enc_loop_func (nat_to_bitstring h, n, h, []) c x) = (c, x)" using enc_loop_func.simps(1) by auto
+  then show ?case using local.Nil(3) by auto
+next
+  case (Cons a m)
+  then have enc_loop_def: "snd (enc_loop_func (nat_to_bitstring h, n, h, (a # m)) c x) = snd(
+        (let x_i = x * x mod n in
+        let p_i = (nat_to_bitstring h) (x_i mod 2^h) in
+        let c_i = a [\<oplus>] p_i in
+        enc_loop_func ((nat_to_bitstring h), n, h, m) (c_i # c) x_i))" using enc_loop_func.simps by auto
+
+  from mod_less_divisor assms(1) have "x * x mod n < n" by auto
+  
+  from this enc_loop_def Cons.IH assms(1) assms(2) 
+  have use_ia: "snd (enc_loop_func (nat_to_bitstring h, n, h, (a # m)) c x) = (x * x mod n) ^ (2 ^ length m) mod n"
+    by metis
+
+  have "(x * x) ^ (2 ^ length m) mod n = (x * x mod n) ^ (2 ^ length m) mod n"  
+    using power_mod[symmetric] by auto
+  from use_ia this have x_times_x:  "snd (enc_loop_func (nat_to_bitstring h, n, h, (a # m)) c x) = (x * x) ^ (2 ^ length m) mod n" 
+    by auto
+
+  have "(x * x) ^ (2 ^ length m) = x ^ (2 ^ length (a # m))"
+    by (auto simp add: power2_eq_square power_mult) 
+  from this x_times_x show ?case by auto
+qed
+
+corollary enc_loop_exp: 
+  assumes "n > 0" "h > 0" "x < n"
+  shows "snd (enc_loop (n, h, m) x) = x ^ (2 ^ (length m)) mod n"
+  by (auto intro: enc_loop_func_exp simp add: assms)
+
+
+lemma same_x_0:
+  assumes 
+    "p mod 4 = 3" "q mod 4 = 3" (*pq_cong_3*)
+    "prime p" "prime q" (*pq_prime*)
+    "r < p * q" 
+  shows "
+    let x = r ^ (t + 1) mod (p * q) in
+    let u_p = x ^ (calculate_exponent t p) in
+    let u_q = x ^ (calculate_exponent t q) in
+    let ((r_p, r_q), _) = euclid_ext p q in
+    nat (u_p * r_p * p + u_q * r_q * q mod (p * q)) = (r * r) mod n"
+proof - 
+
+  show ?thesis sorry
+qed 
+
+theorem 
+  assumes 
+    "p mod 4 = 3" "q mod 4 = 3" (*pq_cong_3*)
+    "prime p" "prime q" (*pq_prime*)
+    "r < n" "m \<noteq> []"
+  shows "decrypt p q (encrypt (p * q) m r) = m"
+proof - 
+  from encrypt_def have "encrypt (p * q) m r = (
+  let h = nat \<lfloor>log 2 (log 2 (p * q))\<rfloor> in 
+  let m_l = split m h in 
+  let (x_0 :: nat) = (r * r) mod (p * q) in 
+  let (c, x_t) = enc_loop (p * q, h, m_l) x_0 in 
+  let x_t' = x_t * x_t mod (p * q) in 
+  (c, x_t'))"
+    by auto
+  then have "fst (encrypt (p * q) m r) 
+  = fst (let h = nat \<lfloor>log 2 (log 2 (p * q))\<rfloor> in 
+  let m_l = split m h in 
+  let x_0 = (r * r) mod (p * q) in enc_loop (p * q, h, m_l) x_0)" 
+    using prod.exhaust prod.sel(1) prod.simps(2)
+    by (metis (mono_tags, lifting))
+
+
+  have "(let h = nat \<lfloor>log 2 (log 2 (real p * real q))\<rfloor> in nat_to_bitstring h) =
+     nat_to_bitstring (nat \<lfloor>log 2 (log 2 (real p * real q))\<rfloor>)" by auto
+  
+
+   show ?thesis sorry
+qed
+
+
+
+text "This formalization, using logarithms makes our proofs harder by introducing real numbers. Now,
+we try to formalize the floor of a logarithm's logarithm without logarithms"
+
+lemma
+  fixes n::nat
+  assumes "n \<ge> 1" "base > (Suc 0)" 
+  shows "floor_nat_log base n = \<lfloor>log base n\<rfloor>"
+  using assms(1)
+proof (induction n rule: dec_induct)
+    
+  case base \<comment> \<open>n = 1\<close>
+
+  have "floor_nat_log base 1 = floor_nat_log_rec base (Suc 0) 0 "  
+    by (auto simp add: floor_nat_log_def )
+  then have "floor_nat_log base 1 
+    = floor_nat_log_rec base ((Suc 0) div base) (Suc 0)"
+    using Suc_less_eq2 floor_nat_log_rec.simps(5) gr0_implies_Suc assms(2)
+    by (metis)
+  also have "(Suc 0) div base = 0" 
+    by (simp add: assms(2)) 
+  moreover have "floor_nat_log base 1 
+    = floor_nat_log_rec base 0 (Suc 0)"
+      using calculation by simp
+  then have  "floor_nat_log base 1  = 0 "
+    using Nat.lessE assms(2) floor_nat_log_rec.simps(4) 
+    by (metis)
+  then show ?case by simp
+next
+  case (step n)
+  have "\<lfloor>log base n\<rfloor> = \<lfloor>ln n / ln base\<rfloor>" by (auto simp add: log_def)
+  
+  
+  then show ?case sorry
+qed
+
+
+lemma "enc_loop (21, 2, [[True, False], [True, False], [True, False]]) 9 = 
+  ([[False, False], [True, True], [False, False]], 18)" 
+  apply (auto simp add: xor_list_def nat_to_bitstring_def nat_to_words_len_def)
+  by (auto simp add: nat_to_words_def)
 
 (* TODO: Clean everything out! E.g. put supporting auxiliary functions to BG_aux.thy.  *)
-(* TODO: Ask about clean coding principles - this seems clunky, is it really ok?*)
 (* TODO: Check if this works as intended! - But how? *)
